Define simulation up-to context

src/opt/Simulation.v
@@ -21,49 +21,61 @@ Inductive sim_memory (mem_src mem_tgt:Memory.t): Prop :=
 .
 
 
-(* TODO: inftau & liveness *)
-Inductive _sim_thread
-          (sim_thread: forall (th1_src:Thread.t) (mem_k_src:Memory.t)
-                         (th1_tgt:Thread.t) (mem_k_tgt:Memory.t), Prop)
-          (th1_src:Thread.t) (mem_k_src:Memory.t)
-          (th1_tgt:Thread.t) (mem_k_tgt:Memory.t): Prop :=
-| sim_thread_terminal
-    (TGT: Thread.is_terminal th1_tgt)
-    (SRC: forall mem1_src
-            (LOCAL: Memory.le th1_src.(Thread.local) mem1_src)
-            (FUTURE: Memory.future mem_k_src mem1_src),
-        exists th2_src mem2_src,
-          <<STEPS: rtc Thread.internal_step (th1_src, mem1_src) (th2_src, mem2_src)>> /\
-          <<TERMINAL: Thread.is_terminal th2_src>>)
-| sim_thread_step
-    (STEP:
-       forall mem1_src mem1_tgt
-         (MEMORY1: sim_memory mem1_src mem1_tgt)
-         (LOCAL_SRC: Memory.le th1_src.(Thread.local) mem1_src)
-         (LOCAL_TGT: Memory.le th1_tgt.(Thread.local) mem1_tgt)
-         (FUTURE_SRC: Memory.future mem_k_src mem1_src)
-         (FUTURE_TGT: Memory.future mem_k_tgt mem1_tgt),
-       forall e th2_tgt mem2_tgt
-         (STEP_TGT: Thread.step e th1_tgt mem1_tgt th2_tgt mem2_tgt),
-       exists th2_src mem2_src,
-         <<STEP_SRC: Thread.step e th1_src mem1_src th2_src mem2_src>> /\
-         <<MEMORY2: sim_memory mem2_src mem2_tgt>> /\
-         <<SIM: sim_thread th2_src mem2_src th2_tgt mem2_tgt>>)
-.
-Hint Constructors _sim_thread.
+Definition SIM_THREAD :=
+  forall (th1_src:Thread.t) (mem_k_src:Memory.t)
+    (th1_tgt:Thread.t) (mem_k_tgt:Memory.t), Prop.
 
+Definition sim_interference
+           (th1_src:Thread.t) (mem_k_src:Memory.t)
+           (th1_tgt:Thread.t) (mem_k_tgt:Memory.t): Prop :=
+  forall mem1_src mem1_tgt
+    (MEMORY1: sim_memory mem1_src mem1_tgt)
+    (LOCAL_SRC: Memory.le th1_src.(Thread.local) mem1_src)
+    (LOCAL_TGT: Memory.le th1_tgt.(Thread.local) mem1_tgt)
+    (FUTURE_SRC: Memory.future mem_k_src mem1_src)
+    (FUTURE_TGT: Memory.future mem_k_tgt mem1_tgt),
+    <<TERMINAL:
+      forall (TERMINAL_TGT: Thread.is_terminal th1_tgt),
+      exists th2_src mem2_src,
+        <<STEPS: rtc Thread.internal_step (th1_src, mem1_src) (th2_src, mem2_src)>> /\
+        <<TERMINAL_SRC: Thread.is_terminal th2_src>>>> /\
+    <<DECLARE:
+      forall (TERMINAL_TGT: th1_tgt.(Thread.local) = Memory.init),
+      exists th2_src mem2_src,
+        <<STEPS: rtc Thread.internal_step (th1_src, mem1_src) (th2_src, mem2_src)>> /\
+        <<TERMINAL_SRC: th2_src.(Thread.local) = Memory.init>>>>.
+
+(* TODO: inftau & liveness *)
+Definition _sim_thread_step
+           (sim_thread: SIM_THREAD)
+           (th1_src:Thread.t) (mem_k_src:Memory.t)
+           (th1_tgt:Thread.t) (mem_k_tgt:Memory.t): Prop :=
+  forall mem1_src mem1_tgt
+    (MEMORY1: sim_memory mem1_src mem1_tgt)
+    (LOCAL_SRC: Memory.le th1_src.(Thread.local) mem1_src)
+    (LOCAL_TGT: Memory.le th1_tgt.(Thread.local) mem1_tgt)
+    (FUTURE_SRC: Memory.future mem_k_src mem1_src)
+    (FUTURE_TGT: Memory.future mem_k_tgt mem1_tgt),
+  forall e th2_tgt mem2_tgt
+    (STEP_TGT: Thread.step e th1_tgt mem1_tgt th2_tgt mem2_tgt),
+  exists th2_src mem2_src,
+    <<STEP_SRC: Thread.step e th1_src mem1_src th2_src mem2_src>> /\
+    <<MEMORY2: sim_memory mem2_src mem2_tgt>> /\
+    <<SIM: sim_thread th2_src mem2_src th2_tgt mem2_tgt>>.
+
+Lemma _sim_thread_step_mon: monotone4 _sim_thread_step.
+Proof.
+  ii. exploit IN; eauto. i. des.
+  eexists _, _. splits; eauto.
+Qed.
+Hint Resolve _sim_thread_step_mon: paco.
+
+Definition _sim_thread R := sim_interference /4\ _sim_thread_step R.
 Lemma _sim_thread_mon: monotone4 _sim_thread.
 Proof.
-  repeat intro; inv IN.
-  - econs 1; eauto.
-  - econs 2. i.
-    exploit STEP; eauto. i. des.
-    eexists _, _. splits; eauto.
+  ii. unfold _sim_thread in IN. des.
+  split; auto. eapply _sim_thread_step_mon; eauto.
 Qed.
 Hint Resolve _sim_thread_mon: paco.
 
-Definition sim_thread: _ -> _ -> _ -> _ -> Prop := paco4 _sim_thread bot4.
-
-Definition sim_thread_init s1 s2 :=
-  sim_thread (Thread.init s1) Memory.init
-             (Thread.init s2) Memory.init.
+Definition sim_thread: SIM_THREAD := paco4 _sim_thread bot4.
