src/opt/Upto4.v
@@ -1,0 +1,128 @@
+Require Import paco4.
+Require Import sflib.
+
+Set Implicit Arguments.
+
+Section Respectful4.
+  Variable T0: Type.
+  Variable T1: forall (x0: @T0), Type.
+  Variable T2: forall (x0: @T0) (x1: @T1 x0), Type.
+  Variable T3: forall (x0: @T0) (x1: @T1 x0) (x2: @T2 x0 x1), Type.
+  Definition rel := rel4 T0 T1 T2 T3.
+
+  Variable gf: rel -> rel.
+  Hypothesis gf_mon: monotone4 gf.
+
+  Inductive sound (clo: rel -> rel): Prop :=
+  | sound_intro
+      (MON: monotone4 clo)
+      (SOUND:
+         forall r (PFIX: r <4= gf (clo r)),
+           r <4= paco4 gf bot4)
+  .
+  Hint Constructors sound.
+
+  Structure respectful (clo: rel -> rel) : Prop :=
+  | respectful_intro
+      (MON: monotone4 clo)
+      (RESPECTFUL:
+         forall l r (LE: l <4= r) (GF: l <4= gf r),
+           clo l <4= gf (clo r)).
+  Hint Constructors respectful.
+
+  Inductive grespectful (r: rel) e1 e2 e3 e4: Prop :=
+  | grespectful_intro
+      clo
+      (RES: respectful clo)
+      (CLO: clo r e1 e2 e3 e4)
+  .
+  Hint Constructors grespectful.
+
+  Lemma gfclo_mon: forall clo, sound clo -> monotone4 (gf <*> clo).
+  Proof. intros; destruct H; eauto using gf_mon. Qed.
+  Hint Resolve gfclo_mon : paco.
+
+  Lemma sound_is_gf: forall clo (UPTO: sound clo),
+      paco4 (gf <*> clo) bot4 <4= paco4 gf bot4.
+  Proof.
+    i. punfold PR. edestruct UPTO.
+    eapply (SOUND (paco4 (gf <*> clo) bot4)); eauto.
+    i. punfold PR0.
+    eapply (gfclo_mon UPTO); eauto.
+    intros. destruct PR1; eauto. done.
+  Qed.
+
+  Lemma respectful_is_sound: respectful <1= sound.
+  Proof.
+    intro clo.
+    set (rclo := fix rclo clo n (r: rel) :=
+           match n with
+           | 0 => r
+           | S n' => rclo clo n' r \4/ clo (rclo clo n' r)
+           end).
+    i. destruct PR. econs; eauto.
+    i. set (rr e1 e2 e3 e4 := exists n, rclo clo n r e1 e2 e3 e4).
+    assert (rr x0 x1 x2 x3) by (exists 0; eauto); clear PR.
+    cut (forall n, rclo clo n r <4= gf (rclo clo (S n) r)).
+    { intro X; revert x0 x1 x2 x3 H; pcofix CIH; i.
+      unfold rr in *; des; eauto 10 using gf_mon. }
+    induction n; i; [by s; eauto using gf_mon|].
+    ss; des; [by eauto using gf_mon|].
+    eapply gf_mon; [eapply RESPECTFUL; [|apply IHn|]|]; inst; s; eauto.
+  Qed.
+
+  Lemma respectful_compose
+        clo1 clo2
+        (RES1: respectful clo1)
+        (RES2: respectful clo2):
+    respectful (clo1 <*> clo2).
+  Proof.
+    i. destruct RES1, RES2.
+    econs.
+    - ii. eapply MON; eauto.
+    - i. eapply RESPECTFUL; [| |apply PR].
+      + i. eapply MON0; eauto.
+      + i. eapply RESPECTFUL0; eauto.
+  Qed.
+
+  Lemma grespectful_respectful: respectful grespectful.
+  Proof.
+    econs; ii.
+    - destructs IN RES; exists clo; eauto.
+    - destructs PR RES; eapply gf_mon with (r:=clo r); eauto.
+  Qed.
+
+  Lemma gfgres_mon: monotone4 (gf <*> grespectful).
+  Proof.
+    destruct grespectful_respectful; eauto using gf_mon.
+  Qed.
+  Hint Resolve gfgres_mon : paco.
+
+  Lemma grespectful_greatest: forall clo (RES: respectful clo), clo <5= grespectful.
+  Proof.
+    eauto.
+  Qed.
+
+  Lemma grespectful_incl: forall r, r <4= grespectful r.
+  Proof.
+    i; eexists (fun x => x); eauto.
+  Qed.
+  Hint Resolve grespectful_incl.
+
+  Lemma grespectful_compose: forall clo (RES: respectful clo) r,
+      clo (grespectful r) <4= grespectful r.
+  Proof.
+    i; eapply grespectful_greatest with (clo := clo <*> grespectful);
+      eauto using respectful_compose, grespectful_respectful.
+  Qed.
+
+  Lemma grespectful_incl_rev: forall r,
+      grespectful (paco4 (gf <*> grespectful) r) <4= paco4 (gf <*> grespectful) r.
+  Proof.
+    intro r; pcofix CIH; i; pfold.
+    eapply gf_mon, grespectful_compose, grespectful_respectful.
+    destruct grespectful_respectful; eapply RESPECTFUL, PR; i; [by eauto using grespectful_incl|].
+    punfold PR0.
+      by eapply gfgres_mon; eauto; i; destruct PR1; eauto.
+  Qed.
+End Respectful4.
